Changed fresh to be function, and proved deterministic

build.hs
@@ -1,11 +1,13 @@
 import Development.Shake
+import Development.Shake.Util
 import Development.Shake.FilePath
+import Data.Maybe
 
 main = shakeArgs shakeOptions $ do  
   want ["compiler.vo"]
   "*.vo" %> \out -> do
     let source = out -<.> ".v"
     deps <- cmd $ "coqdep -I . " ++ source 
-    need $ drop 3 $ words $ fromStdout deps
+    need $ fromMaybe [] $ lookup out $ parseMakefile $ fromStdout deps
     cmd $ "coqc " ++ source
   phony "clean" $ removeFilesAfter "." ["//*.vo", "//*.glob"]
