cbn.v
@@ -1,24 +1,25 @@
 (* Based on figure 8 of ariola et al *) 
-Require Import Lists.List Decidable CpdtTactics Program.Basics.
+Require Import Lists.List EqNat Decidable CpdtTactics Program.Basics.
 Require Import Unicode.Utf8_core.
 Require Import expr util.
 Require Import Arith.Peano_dec.
 
 Definition heap := list (nat * tm). 
 
-Inductive configuration : Type := 
-  | st : heap -> tm -> configuration.
+Record configuration : Type := st {
+  st_heap : heap;
+  st_tm : tm
+}.
 
 Notation " x ↦ M " := (x, M) (at level 40).
 Notation " ⟨ Φ ⟩ m " := (st Φ m) (at level 40).
 Notation " ⟨ Ψ , b ⟩ N " := (st (cons b Ψ) N) (at level 40).
 Notation " ⟨ Φ , b , Ψ ⟩ N " := (st (Datatypes.app Ψ (cons b Φ)) N) (at level 40).
 
-Definition fresh (n : nat) (e : tm) (h : heap) := 
-  ~ In n (vars e) 
-  ∧ ~ In n (domain h).
-
 Definition I (e : tm ) : configuration := st nil e.
+
+Definition fresh' {A} (x: nat) (Φ : Map nat A) :=
+  ∃ p, fresh Φ = exist (isfresh Φ) x p. 
 
 (* Direct description of Maraist et al. Figure 8, with amendment from  *)
 Reserved Notation " c1 '⇓' c2 " (at level 50).
@@ -27,7 +28,7 @@ Inductive step : configuration → configuration → Prop :=
             ⟨Φ, x ↦ M, Υ⟩var x ⇓ ⟨Ψ, x ↦ :λy,N, Υ⟩:λy,N
   | Abs : ∀ N x Φ,  ⟨Φ⟩:λx,N ⇓ ⟨Φ⟩:λx,N
   | App : ∀ M N L B y x x' Φ Ψ Υ,
-              fresh x' N Φ → 
+              fresh' x' Ψ → 
             ⟨Φ⟩L ⇓ ⟨Ψ⟩:λx,N → 
         ⟨Ψ, x' ↦ M⟩[var x'//x]N ⇓ ⟨Υ⟩:λy,B →
            ⟨Φ⟩(L@M) ⇓ ⟨Υ⟩:λy,B
@@ -41,7 +42,7 @@ Definition closed_under (c : configuration) : Prop := match c with
 
 Definition closed (t : tm) : Prop := closed_under (st nil t).
 
-Definition well_formed_heap (h : heap) : Prop := forevery h (λ p, match p with
+Definition well_formed_heap (h : heap) : Prop := unique (domain h) ∧ forevery h (λ p, match p with
   | (x, M) => closed_under (st h M)
   end).
 
@@ -52,7 +53,7 @@ Definition well_formed (c : configuration) : Prop := match c with
 Lemma well_formed_app : ∀ (Φ Ψ:heap) (x:nat) (M N:tm), 
   well_formed (⟨Φ, x ↦ M, Ψ⟩N) →
   well_formed (⟨Φ, x ↦ M, Ψ⟩M).
-intros. destruct H. clear H. split. unfold well_formed_heap in H0. apply
+intros. destruct H. clear H. split. unfold well_formed_heap in H0. destruct H0. apply
 forevery_inf in H0. assumption. auto. Qed. 
 
 Lemma well_formed_app' : ∀ (Φ Ψ:heap) (x:nat) (M N:tm), 
@@ -64,10 +65,14 @@ unfold well_formed_heap in H0. unfold closed_under in H0. rewrite domain_inf
 with (m:=N) (m':=M). rewrite forevery_app. rewrite forevery_app in H0. destruct
 H0. split. crush. crush. Qed.
 
-Definition stheap (c:configuration) : heap := match c with | st h t => h end.
-Definition sttm (c:configuration) : tm := match c with | st h t => t end.
+Lemma unique_step : ∀ s s', unique (domain (st_heap s)) → step s s' → unique
+(domain (st_heap s')). 
+intros. induction H0. simpl. simpl in IHstep. rewrite <- domain_inf with (m:=M).
+apply IHstep. assumption. assumption. simpl. simpl in IHstep2. simpl in IHstep1.
+apply IHstep2. simpl in H. apply ucons. unfold fresh' in H0. destruct H0.
+assumption. apply IHstep1. assumption. Qed. 
 
-Lemma not_vars_fvs : forall n e, ~(In n (vars e)) -> ~(In n (fvs e)).
+Lemma not_vars_fvs : ∀ n e, ~(In n (vars e)) -> ~(In n (fvs e)).
 induction e. simpl. intros. assumption. simpl. rewrite in_app_iff. rewrite
 in_app_iff. intros. apply not_or in H. destruct H. apply IHe1 in H. apply IHe2
 in H0. unfold not. intros. destruct H1. apply H in H1. assumption. apply H0 in
@@ -76,24 +81,7 @@ unfold not. intros. unfold not in H. assert (n <> n0). unfold not. intros.
 symmetry in H2.  apply H in H2. assumption. apply remove_not_in with (ns:=fvs e)
 in H2. apply H2 in H1. apply H0 in H1. assumption. Qed.  
 
-Lemma fresh_subst : forall x x' e h, fresh x' e h -> fvs ([x'//x]e) = replace x x' (fvs e).
-(* Var *)
-intros. destruct H. clear H0. induction e. destruct (eq_nat_dec x n). subst.
-simpl. unfold replace'. rewrite eq_nat_dec_refl. reflexivity. simpl. unfold
-replace'. rewrite eq_nat_dec_neq with (p := n0). reflexivity.
-(* App *)
-simpl in H. simpl. rewrite in_app_iff in H. apply not_or in H. destruct H. 
-apply IHe1 in H. apply IHe2 in H0. rewrite H. rewrite H0. unfold replace.
-rewrite map_app. reflexivity.
-(* Lam *)
-simpl in H. apply not_or in H. destruct H. assert (~ In x' (fvs e)). apply
-not_vars_fvs. assumption. apply IHe in H0. simpl. destruct
-(eq_nat_dec x n). simpl. subst. rewrite replace_remove. reflexivity. 
-simpl. rewrite H0. rewrite remove_replace_comp. reflexivity. assumption.
-assumption. unfold not. intros. rewrite H2 in n0. assert (x = x). reflexivity.
-apply n0 in H3. assumption. Qed.
-
-Lemma monotonic_heap : ∀ c1 c2, c1 ⇓ c2 → domain (stheap c1) ⊆ domain (stheap c2).  
+Lemma monotonic_heap : ∀ c1 c2, c1 ⇓ c2 → domain (st_heap c1) ⊆ domain (st_heap c2).  
 intros c1 c2 step.  induction step. simpl. simpl in IHstep. 
 unfold domain at 2. unfold domain at 2 in IHstep. rewrite map_app. rewrite
 map_app in IHstep.  simpl. simpl in IHstep. assumption. 
@@ -106,15 +94,39 @@ well_formed_app' in H. assumption. assumption. apply IHstep2.
 simpl in H. destruct H. rewrite app_subset_and in H. destruct H. assert
 (well_formed (⟨Φ ⟩ L)). split; assumption. apply IHstep1 in H3. clear IHstep2. 
 split. Focus 2. unfold well_formed_heap. simpl. split. assert (subset (domain Φ)
-(domain Ψ)). apply monotonic_heap in H0_. assumption. apply subset_trans with
-(ys := (domain Φ)) (zs:= (domain Ψ)) in H2. apply subset_cons. assumption.
-assumption. unfold well_formed in H3. destruct H3. unfold well_formed_heap in
-H4. unfold closed_under in H4. apply forevery_impl with (p:=(λ p:nat*tm, let
-(_,M0) := p in subset (fvs M0) (domain Ψ))). intros. destruct a. apply
-subset_cons. assumption. assumption. simpl. simpl in H3. destruct H3. assert
-(subset (fvs ([x' // x]N)) (fvs x' ++ remove x (fvs N))).  apply subst_subset.
-simpl in H5. apply (cons_subset x') in H3. apply subset_trans with
-(ys:=x'::remove x (fvs N)). assumption. assumption. Qed. 
+(domain Ψ)). apply monotonic_heap in H0_. assumption. destruct H3. apply ucons.
+unfold fresh' in H0. destruct H0.  assumption. destruct H5. assumption. split.
+apply subset_cons. apply monotonic_heap in H0_. simpl in H0_. apply subset_trans
+with (ys := (domain Φ)) (zs:= (domain Ψ)) in H2; assumption.  unfold well_formed
+in H3. destruct H3. unfold well_formed_heap in H4. unfold closed_under in H4.
+apply forevery_impl with (p:=(λ p:nat*tm, let (_,M0) := p in subset (fvs M0)
+(domain Ψ))). intros. destruct a. apply subset_cons. assumption. destruct H4.
+assumption. simpl. simpl in H3. destruct H3. assert (subset (fvs ([x' // x]N))
+(fvs x' ++ remove x (fvs N))).  apply subst_subset.  simpl in H5. apply
+(cons_subset x') in H3. apply subset_trans with (ys:=x'::remove x (fvs N)).
+assumption. assumption. Qed. 
+
+Lemma det_step : ∀ a b c, well_formed a → a ⇓ b → a ⇓ c → b = c. 
+intros a b c wf s. generalize dependent c. induction s. apply well_formed_app in
+wf. specialize (IHs wf). intros. inversion H. subst. symmetry in H0. apply
+unique_inf in H0; try (destruct wf; destruct H2; assumption). destruct H0.
+destruct H1. subst. apply IHs in H3. inversion H3. subst. apply app_eq_l in H1.
+inversion H1.  subst. reflexivity. intros. inversion H. subst. auto. inversion 
+wf. simpl in H0. rewrite app_subset_and in H0. destruct H0. specialize (IHs1
+(conj H0 H1)). assert (s1':=s1). apply well_formed_step in s1; try (apply (conj
+H0 H1)). destruct s1. assert (s1:=s1'). simpl in H3. apply monotonic_heap in s1.
+simpl in s1. apply subset_trans with (xs:=fvs M) in s1; try assumption. assert
+(well_formed_heap (x' ↦ M :: Ψ)). split. simpl. apply ucons. destruct H.
+assumption. inversion H4. assumption. simpl. split. apply subset_cons.
+assumption. inversion H4. unfold closed_under in H6. apply forevery_impl with
+(p:=λ p, let (_,M0) := p : nat * tm in fvs M0 ⊆ domain Ψ). intros. destruct a.
+apply subset_cons. assumption. assumption. assert (fvs ([x'//x]N) ⊆ (x'::domain Ψ)).
+apply subset_trans with (ys:=fvs (var x') ++ remove x (fvs N)). apply
+subst_subset. simpl. split. apply or_introl. reflexivity. apply subset_cons.
+assumption. assert (well_formed (⟨Ψ, x' ↦ M⟩[x'//x]N)). split. assumption.
+assumption. specialize (IHs2 H7). intros. inversion H8. subst. apply IHs1 in
+H14. inversion H14. subst. destruct H12. inversion H9. destruct H. rewrite H in
+H9. inversion H9. subst. apply IHs2 in H15. assumption. Qed. 
 
 (* Collapsing configuration to term 
 Fixpoint collapse (h : heap) : tm → tm :=  match h with
