cem.v
@@ -5,8 +5,10 @@ Require Import CpdtTactics.
 
 Definition append := Datatypes.app.
 
-Inductive closure : Type := 
-  | close : tm → nat → closure. 
+Record closure : Type := close {
+  clos_tm : tm;
+  clos_env : nat
+}.
 
 Inductive cell : Type :=
   | cl : closure → nat → cell.
@@ -34,12 +36,6 @@ Inductive cactus_lookup : nat → nat → heap → nat → Prop :=
   | pred : forall x y z Φ M Υ i, cactus_lookup i x Φ z → 
             cactus_lookup (S i) y (Φ ++ (y ↦ {M, x}):: Υ) z.
 
-Definition lookup {a} (x:nat) (l:list (nat * a)) : option a := 
-  match find (λ p, beq_nat x (fst p)) l with 
-    | None => None
-    | Some (k,v) => Some v
-  end.
-
 Fixpoint clu (v env:nat) (h:heap) : option (nat * closure) := match lookup env h with
   | None => None
   | Some (cl c a) => match v with
@@ -48,8 +44,8 @@ Fixpoint clu (v env:nat) (h:heap) : option (nat * closure) := match lookup env h
     end
   end.
 
-Definition fresh (n : nat) (h : heap) := 
-  ~ In n (domain h).
+Definition isfresh (h : heap) (n : nat) : Prop := ¬ In n (domain h). 
+Axiom fresh : ∀ h:heap, @sig nat (isfresh h). 
 
 Definition closed_under (c : closure) (h : heap)  : Prop := match c with
   | close t e => forevery (fvs t) 
@@ -71,7 +67,8 @@ Inductive step : configuration → configuration → Prop :=
             ⟨Φ, (x ↦ {M,y}), Υ⟩M ⇓ ⟨Ψ, (x ↦ {M,y}), Υ⟩close (:λB) e →
     ⟨Φ, x ↦ {M, y}, Υ⟩close (var v) z ⇓ ⟨Ψ, x ↦ {close (:λB) e, y}, Υ⟩close (:λB) e
   | Abs : ∀ N Φ e, ⟨Φ⟩close (:λN) e ⇓ ⟨Φ⟩close (:λN) e
-  | App : ∀ N M B B' Φ Ψ Υ f e ne ae, fresh f Ψ → 
+  | App : ∀ N M B B' Φ Ψ Υ f e ne ae p, 
+                fresh Ψ = exist (isfresh Ψ) f p → 
           ⟨Φ⟩close M e ⇓ ⟨Ψ⟩close (:λB) ne → 
       ⟨Ψ, f ↦ {close N e, ne}⟩close B f ⇓ ⟨Υ⟩close (:λB') ae   →
               ⟨Φ⟩close (M@N) e ⇓ ⟨Υ⟩close (:λB') ae
@@ -84,16 +81,33 @@ Definition step' (c1 c2: configuration') : Prop := match (c1, c2) with
 Lemma well_formed_inf : ∀ c x c' n  Φ Υ, 
   well_formed (⟨Φ, x ↦ cl c' n, Υ⟩c) → 
   well_formed (⟨Φ, x ↦ cl c' n, Υ⟩c').
-  intros. split. inversion H. unfold well_formed_heap in H1. apply forevery_app in H1.
-  destruct H1. simpl in H2. destruct H2. auto. 
-  auto. inversion H. auto. Qed. 
+intros. split. inversion H. unfold well_formed_heap in H1. apply forevery_app in H1.
+destruct H1. simpl in H2. destruct H2. auto. 
+auto. inversion H. auto. Qed. 
+
+Lemma forevery_cons {A} : ∀ (p:A→Prop) (x:A) xs, p x → forevery xs p → forevery (x::xs) p. 
+intros. simpl. split; assumption. Qed. 
 
 (*
+
+Lemma closed_under_inf' : ∀ c c' e x Ψ Φ, closed_under c (Φ ++ x ↦ {c', e} :: Ψ) →
+  closed_under c (Φ ++ x ↦ {c, e} :: Ψ).
+intros. unfold closed_under. destruct c. unfold closed_under in H. induction (fvs clos_tm0). simpl. auto.
+simpl. split. simpl in H. destruct H. destruct H. destruct H. destruct H.
+destruct (clu a clos_env0 (Φ ++ x ↦ {c', e} :: Ψ)). destruct p. inversion H.
+destruct c. destruct = 
+destruct H. 
+apply
+ex_intro with x0. apply ex_intro with x1. split. destapply forevery_inf with (xs:=Φ)
+(ys:=Ψ) (y:=x ↦ {, e}). . .  forevery_app in H. 
+
 Lemma well_formed_inf' : ∀ Φ Ψ x c c' n,
   well_formed (⟨Φ, x ↦ cl c' n, Ψ⟩c) →
   well_formed (⟨Φ, x ↦ cl c n, Ψ⟩c).
-intros. split.  inversion H. apply forevery_app in H1. destruct H1. unfold
-closed_under. destruct c. unfold closed_under in H0. simpl in H2. destruct H2. 
+intros. split.  inversion H. apply forevery_app in H1. destruct H1. simpl in H2. destruct H2. rename x into X. apply forevery_cons
+with (x:=X ↦ {c', n}) (xs:=Φ) in H0. assumption. apply  . assumption.  in H0. assert (conj H0 H3). forevery (x ↦ {c, n} :: Φ), λ
+x0, match x0 with _ ↦ {c1, _} => closed_under c1 (append (nat * cell) Ψ (x ↦ {c',
+n} :: Φ)) end). 
 unfold closed_under. rewrite forevery_app.  with (m:=n) (m':=n). assumption.
 unfold well_formed_heap. unfold closed_under.  unfold well_formed_heap in H0.
 unfold closed_under in H0. rewrite domain_inf with (m:=N) (m':=M). rewrite
