cem_cesm.v
@@ -1,54 +1,186 @@
-Require Import cem cesm.
+Require Import cem cesm util.
 Require Import Unicode.Utf8.
 Require Import relations. 
 Require Import List. 
 
-Notation " c1 '→_s*' c2 " := (refl_trans_clos step' c1 c2) (at level 30). 
-
 Definition b2s (c : configuration) : stack → state := match c with
   | conf h c => λ s, st h s c end.
 
-Definition convert_to_cesm (c c' : configuration) : Prop := match (c, c') with
-  | (conf h c, conf h' c') => ∀ s, (st h s c) →_s* (st h' s c') end.
+Notation " c1 '↦s*' c2 " := (c1 →s* c2 ∧ state_value c2) (at level 30). 
 
-Lemma cem_cesm : ∀ c v, c ⇓ v → ∀ s, b2s c s →_s* b2s v s. 
+Definition convert_to_cesm (c c' : configuration) : Prop := match (c, c') with
+  | (conf h c, conf h' c') => ∀ s, (st h s c) →s* (st h' s c') end.
+
+Lemma cem_cesm : ∀ c v, c ⇓ v → ∀ s, b2s c s →s* b2s v s. 
 (* Var *)
 intros c v H. induction H. simpl. simpl in IHstep. 
 assert (∀ s, step' (st (Υ ++ (x ↦ {M,y} :: Φ)) s (close (db.var v) z)) 
                    (st (Υ ++ (x ↦ {M,y} :: Φ)) (inr x::s) M)).
-intros. apply Var. assumption. 
+intros. apply Var'. assumption. 
 assert (∀ s, step' (st (Υ ++ x ↦ {M, y} :: Ψ) (inr x :: s) (close (db.lam B) e))
                    (st (Υ ++ x ↦ {close (db.lam B) e, y} :: Ψ) s (close (db.lam B) e)))
 .
 apply Upd. 
 intros. rename y into Y.  
-apply t_step with (y:=[Υ ++ x ↦ {M, Y} :: Φ, inr x :: s]M). auto. 
-apply t_step2 with (y:= [Υ ++ x ↦ {M, Y} :: Ψ, inr x :: s](close (db.lam B) e)). 
+apply t_step with (y:=[Υ ++ x ↦ {M, Y} :: Φ, inr x :: s | M]). auto. 
+apply t_step2 with (y:= [Υ ++ x ↦ {M, Y} :: Ψ, inr x :: s | (close (db.lam B) e)]). 
 auto. auto.   
 (* Lam *)
 intros. apply t_refl. 
 (* App *)
 intros. apply t_step with (y:=b2s (⟨Φ ⟩ close M e) (inl (close N e)::s)). 
-apply App. 
+apply App'. 
 apply refl_trans_clos_app with (y:=b2s (⟨Ψ, f ↦ {close N e, ne} ⟩ close B f) s).
 apply t_step2 with (y:=b2s (⟨Ψ ⟩ close (db.lam B) ne) (inl (close N e):: s)).
-simpl. rename e into E. rename s into S. apply Abs with (b:=B) (e:=ne)
+simpl. rename e into E. rename s into S. apply Abs' with (b:=B) (e:=ne)
 (c:=close N E) (s:= S) in H.  
 assumption.
 auto. 
 auto. 
 Qed. 
 
+Lemma cem_cesm_nf : ∀ c v Φ Ψ, conf Φ c ⇓ conf Ψ v → st Φ nil c ↦s* st Ψ nil v. 
+intros. split. apply cem_cesm with (s:=nil) in H. simpl in H. assumption.
+inversion H; unfold state_value; split;  try (apply db.val); reflexivity. Qed.
+
 Definition s2b (s : state) : configuration := match s with
   | st h s c => conf h c
   end.
 
-Definition st_stack := λ s, match s with
-  | st h s c => s
-  end.
+Lemma step_stack_app : ∀ a b z c c' Φ Ψ, st Φ a c →s st Ψ b c'
+                                      → st Φ (a++z) c →s st Ψ (b++z) c'. 
+intros. inversion H; try constructor. assumption. rename p into P. apply Abs'
+with (p:=P). assumption. Qed. 
 
+Lemma step_stack_app' : ∀ a b z c c' Φ Ψ, st Φ (a++z) c →s st Ψ (b++z) c'
+                                             → st Φ a c →s st Ψ b c'. 
+intros. inversion H; subst. rewrite app_comm_cons in H2. apply app_eq_r in H2.
+subst. constructor. rewrite app_comm_cons in H5. apply app_eq_r in H5. subst.
+apply Var'. assumption. rewrite app_comm_cons in H2. apply app_eq_r in H2. subst.
+apply Abs' with (p:=p). assumption. rewrite app_comm_cons in H5. apply app_eq_r
+in H5. subst. constructor. Qed.  
 
+Lemma rtc_step_stack_app : ∀ a b z c c' Φ Ψ, st Φ a c →s* st Ψ b c'
+                                    → st Φ (a++z) c →s* st Ψ (b++z) c'. 
+intros. remember (st Φ a c). remember (st Ψ b c'). generalize dependent Φ.
+generalize dependent Ψ. generalize dependent a. generalize dependent c.
+generalize dependent c'. generalize dependent b. generalize dependent z.
+induction H; intros; subst. inversion Heqs. subst. apply t_refl. specialize
+(IHrefl_trans_clos z0 b c'). inversion H; subst. specialize (IHrefl_trans_clos
+(close (db.lam b0) e) s Ψ eq_refl (Φ0 ++ l ↦ (cl (close (db.lam b0) e) e') ::
+Υ) eq_refl). apply t_step with (y:=st (Φ0 ++ l ↦ (cl (close (db.lam b0) e) e') ::
+Υ) (s++z0) (close (db.lam b0) e)). apply step_stack_app with (z:=z0) in H.
+assumption. assumption. apply step_stack_app with (z:=z0) in H. specialize 
+(IHrefl_trans_clos c0 (inr l :: a) Ψ eq_refl Φ eq_refl). apply t_step with
+(y:=st Φ (inr l :: a ++ z0) c0). assumption. assumption. specialize
+(IHrefl_trans_clos (close b0 f) s Ψ eq_refl (f ↦ (cl c0 e) :: Φ) eq_refl). apply
+step_stack_app with (z:=z0) in H. apply t_step with (y:=st ((f,cl c0 e) :: Φ) (s
+++ z0) (close b0 f)). assumption. assumption. specialize (IHrefl_trans_clos
+(close m e) (inl (close n e) :: a) Ψ eq_refl Φ eq_refl). apply step_stack_app
+with (z:=z0) in H. apply t_step with (y:=st Φ (inl (close n e) :: a ++ z0)
+(close m e)). assumption. assumption. Qed.
+
+Lemma rtc_step_stack_app' : ∀ a b z c c' Φ Ψ, st Φ (a++z) c →s* st Ψ (b++z) c'
+                                    → st Φ a c →s* st Ψ b c'. 
+intros. remember (st Φ (a++z) c). remember (st Ψ (b++z) c'). generalize
+dependent a. generalize dependent Φ. generalize dependent c.  generalize
+dependent Ψ. generalize dependent c'. generalize dependent b. generalize
+dependent z. induction H; intros; subst. inversion Heqs; subst; clear Heqs.
+apply app_eq_r in H1. subst. apply t_refl. destruct y. specialize
+(IHrefl_trans_clos z0 b c' Ψ eq_refl st_closure st_heap). inversion H; subst.
+destruct a. simpl in H3.  subst. simpl in H. assert (inr l :: st_stack = ((inr l
+:: nil) ++ st_stack)).  auto. rewrite H1 in H. clear H1. replace st_stack
+with (nil++st_stack) in H; auto.  auto.  rewrite (st_stack = nil
+++ st_stack) by auto in H. in H by auto. . .  rewrite <- app_comm_cons in H. 
+apply step_stack_app' in H. 
+simpl in H. subst. apply st_step. 
+IHrefl_trans_clos.   
+
+(* This is much harder, need induction so that  *) 
+Lemma cesm_cem : ∀ Φ c Ψ v, st Φ nil c ↦s* st Ψ nil v  
+                             → conf Φ c ⇓ conf Ψ v.
+(* Induction on steps *)
 (*
-Lemma cesm_cem : ∀ c c' v, c →_s c' → c' →_s* v → st_stack c = st_stack v → s2b c ⇓ s2b v.
-intros. induction H0. induction H. simpl in H1. inversion v. induction H1. 
+intros. remember (st Φ nil c). remember (st Ψ nil v).
+generalize dependent c.  generalize dependent Φ. generalize dependent v.
+generalize dependent Ψ.  destruct H. induction H; intros; subst. inversion
+Heqs. subst. inversion H0. inversion H. destruct v. simpl in H3. subst. apply
+Abs. specialize (IHrefl_trans_clos H0 Ψ v Φ c). remember
+(st Ψ s v). generalize dependent s. generalize dependent H0. generalize
+dependent c. generalize dependent Ψ. generalize dependent v. generalize
+dependent Φ. rewrite rtc_eq in H1. induction H1; intros; subst. inversion H.
+apply cons_neq in H6. inversion H6. symmetry in H6. apply cons_neq in H6.
+inversion H6. apply cons_neq in H6. inversion H6. symmetry in H6. apply cons_neq
+in H6. inversion H6. rewrite <- rtc_eq in H1. clear IHrefl_trans_clos'. subst. apply induction induction
+H1. inversion clear H0.
+inversion H; subst. remember (st Ψ nil v). generalize dependent Ψ. induction H1;
+intros; subst. inversion H. inversion H0; subst.  inversion H; subst. inversion
+generalize dependent v.
+rewrite <- 
+
+specialize
+(IHrefl_trans_clos H0 Ψ v eq_refl). inversion H; intros; subst. remember (st Φ
+(inr l :: nil) c0). remember (st Ψ nil v). generalize
+dependent Ψ. generalize dependent c0. generalize dependent l. generalize dependent Φ. generalize
+dependent v. generalize dependent v0. generalize dependent H0. generalize dependent e. rewrite rtc_eq in
+H1. induction H1; intros; subst. inversion Heqs0. rewrite <- rtc_eq in H1.
+remember (st Φ (inr l :: nil) c0). generalize dependent Φ. generalize dependent
+c0. induction H1. specialize
+(IHrefl_trans_clos H0 v Φ). inversion H0. subst.
+ specialize (IHrefl_trans_clos Ψ v).
+inversion Heqs. 
+sbuispecialize
+(IHrefl_trans_clos Φ c0). remember 
+
+inversion H0. inversion H2. destruct v.
+simpl in H5. subst. specialize IHrefl_trans_clos with (v0:=v).  
+intros. inversion H. subst. inversion H1. destruct v. simpl. destruct
+st_closure. simpl in H3. subst. apply Abs. subst. rewrite rtc_eq in H3. 
+induction H3. inversion H2. subst. simpl. simpl in H0.
+symmetry in H0. apply l_cons_neq in H0. inversion H0. simpl. subst. simpl in H0.
+apply l_cons_neq in H0. inversion H0. subst. simpl in H0. symmetry in H0. apply
+l_cons_neq in H0. inversion H0. subst. simpl in H0. apply l_cons_neq in H0.
+inversion H0. subst.  destruct st_closure. inversion H1. simpl in H5. subst.
+clear H1. clear H3.  simpl in H2. subst. simpl in H0. apply Abs. rewrite rtc_eq
+in H2. destruct H2.  subst. 
+
+subst.induction H. destruct x. destruct
+st_closure. simpl in H0. inversion H1. destruct H. inversion H2. simpl in H. simpl. inversion H. subst. apply Abs. 
+
+
+Lemma cesm_nil : ∀ c v, c →s* v → st_stack c = nil → st_stack v = nil 
+      → ∀ s, (st (st_heap c) s (st_closure c)) →s* (st (st_heap v) s (st_closure v)).
+intros. inversion H. subst. apply t_refl. rewrite rtc_eq in H3. destruct H3. inversion
+H2. subst. simpl in H0. inversion H0. subst. simpl in H1. inversion H1. subst.
+simpl in H0. inversion H0. subst. simpl in H1. inversion H1. rewrite <- rtc_eq
+in H3. destruct c. destruct z0. simpl in H0. simpl in H1. subst.  simpl.
+
+destruct x0. destruct y. inversion H2. subst. inversion H3. subst. induction s. subst. destruct c. destruct z0. simpl. simpl in H0. simpl in
+H1. subst. assumption. subst. 
+duction H3. subst. apply t_step. subst. apply inversion H1. 
+
+                                                ↔ 
+                                          twostep c v.
+intros. split; intros. induction H. induction H. apply ts_refl. 
+:
+
+Lemma push_lam : ∀ xs ys, state Φ nil c →s state 
+
+
+
+assumption. 
+destruct z.
+destruct simpl in
+IHrefl_trans_clos. induction H. 
+simpl. simpl in
+induction H. 
+destruct x. destruct H. destruct H. induction H. destruct x. simpl in H.  destruct st_closure. destruct clos_tm.
+inversion H0. apply cem.Abs. inversion H0. destruct H. 
+destruct H. destruct x. destruct c. destruct t. simpl in
+H0. destruct H1. clear H0. apply  
+H1. splitinversion x. inversion H2. inversion H3. unfold normal_form in H0. induction H. destruct c. simpl in H1. symmetry in H1. apply l_cons_neq in
+H1. inversion H1. simpl in H1. apply l_cons_neq in H1. inversion H1. simpl in
+H1. symmetry in H1. apply l_cons_neq in H1. inversion H1. simpl in H1. apply
+l_cons_neq in H1. inversion H1. induction j
 *)
+
