cesm.v
@@ -2,18 +2,25 @@ Require Import Arith.EqNat.
 Require Import List Unicode.Utf8.
 Require Import Arith.Peano_dec.
 Require Import CpdtTactics.
+Require Import Coq.Init.Specif.
 Require Import db util.
-Require Import cem.
+Require Import cem relations.
 
 Definition stack := list (closure + nat).
 
-Inductive state : Type :=
-  | st : heap → stack → closure → state.
+Record state : Type := st {
+  st_heap : heap;
+  st_stack : stack;
+  st_closure : closure
+}.
+
+Definition state_value (s : state) : Prop := 
+  value (clos_tm (st_closure s)) ∧ st_stack s = nil.
 
 Definition I (e : tm) : state := st nil nil (close e 0).
 
 Notation " x ↦ M " := (x, M) (at level 40).
-Notation " [ Φ , s ] m " := (st Φ s m) (at level 40).
+Notation " [ Φ , s | m ] " := (st Φ s m) (at level 80).
 
 Definition closed (t : tm) : Prop := closed_under (close t 0) nil. 
 
@@ -32,21 +39,106 @@ Definition replaceClosure (l:nat) (c:closure) : nat * cell → nat * cell :=
     | (l', cl c' e) => if eq_nat_dec l l' then (l, cl c e) else x
     end.
 
-Reserved Notation " c1 '→_s' c2 " (at level 50).
+Reserved Notation " c1 '→s' c2 " (at level 50).
 Inductive step' : state → state → Prop :=
   | Upd : ∀ Φ Υ b e e' c l s, 
-  st (Φ++(l,(cl c e'))::Υ) (inr l::s) (close (lam b) e) →_s 
+  st (Φ++(l,(cl c e'))::Υ) (inr l::s) (close (lam b) e) →s 
   st (Φ++(l,(cl (close (lam b) e) e'))::Υ) s (close (lam b) e)
-  | Var : ∀ Φ s v l c e, clu v e Φ = Some (l,c) → 
-  st Φ s (close (var v) e) →_s st Φ (inr l::s) c
-  | Abs : ∀ Φ b e f c s, fresh f Φ → 
-  st Φ (inl c::s) (close (lam b) e) →_s st ((f, cl c e):: Φ) s (close b f)
-  | App : ∀ Φ e s n m, 
-  st Φ s (close (app m n) e) →_s st Φ (inl (close n e)::s) (close m e)
-where " c1 '→_s' c2 " := (step' c1 c2).
+  | Var' : ∀ Φ s v l c e, clu v e Φ = Some (l,c) → 
+  st Φ s (close (var v) e) →s st Φ (inr l::s) c
+  | Abs' : ∀ Φ b e f c s p, fresh Φ = exist (isfresh Φ) f p  → 
+  st Φ (inl c::s) (close (lam b) e) →s st ((f, cl c e):: Φ) s (close b f)
+  | App' : ∀ Φ e s n m, 
+  st Φ s (close (app m n) e) →s st Φ (inl (close n e)::s) (close m e)
+where " c1 '→s' c2 " := (step' c1 c2).
+
+Reserved Notation " c1 '→s2' c2 " (at level 50).
+Inductive step2 : state → state → Prop :=
+  | Upd2 : ∀ Φ c' e' l b e s, 
+  lookup l Φ = Some (cl c' e') →
+  st Φ (inr l::s) (close (lam b) e)  →s2
+  st (replace beq_nat l (cl (close (lam b) e) e') Φ) s (close (lam b) e)
+  | Var2 : ∀ Φ s v l c e, 
+  clu v e Φ = Some (l,c) → 
+  st Φ s (close (var v) e) →s2 st Φ (inr l::s) c
+  | Abs2 : ∀ Φ b e f c s p, 
+  fresh Φ = exist (isfresh Φ) f p  → 
+  st Φ (inl c::s) (close (lam b) e) →s2 st ((f, cl c e):: Φ) s (close b f)
+  | App2 : ∀ Φ e s n m, 
+  st Φ s (close (app m n) e) →s2 st Φ (inl (close n e)::s) (close m e)
+where " c1 '→s2' c2 " := (step2 c1 c2).
+
+Lemma unique_step : ∀ a b, unique (domain (st_heap a)) → a →s b → 
+  unique (domain (st_heap b)). 
+intros. destruct H0; simpl in H; simpl; try assumption. rewrite domain_inf with
+(m' := {c, e'}). assumption. apply ucons. assumption. assumption. Qed. 
+
+Lemma step2_determ : deterministic step2. 
+unfold deterministic. intros. inversion H. inversion H0. subst. inversion
+H5. subst. rewrite H1 in H4. inversion H4. subst. reflexivity. subst. inversion
+H5. subst. inversion H5. subst. inversion H4. subst. inversion H0. subst.
+rewrite H1 in H7. inversion H7. subst. reflexivity. subst. inversion H0; subst.
+rewrite H1 in H8. inversion H8. subst. reflexivity. subst. inversion H0. subst.
+reflexivity. Qed. 
+
+Notation " c1 '→s*' c2 " := (refl_trans_clos step' c1 c2) (at level 30). 
+Definition normalize (c1 c2 : state) := refl_trans_clos step' c1 c2 ∧ state_value c2.
+Definition normalize2 (c1 c2 : state) := refl_trans_clos step2 c1 c2 ∧ state_value c2.
+Notation " c1 '↦s*' c2 " := (normalize c1 c2) (at level 30). 
+
+Lemma normalize2_determ : deterministic normalize2.  
+unfold deterministic. intros. destruct H. induction H. destruct H0. induction H.
+reflexivity. inversion H; subst. inversion H1; subst. simpl in H5.  inversion
+H5. inversion H. subst. inversion H1. inversion H4. inversion H1. inversion H5.
+inversion H1. inversion H3. apply IHrefl_trans_clos. assumption. destruct H0.
+destruct H0. inversion H; subst.  inversion H3. inversion H5. inversion H3.
+inversion H4. inversion H3. inversion H5. inversion H3. inversion H0. apply
+(step2_determ x y y0) in H. subst. split; assumption. assumption. Qed.
+
+Lemma step'_step2 : ∀ s s', unique (domain (st_heap s)) → step' s s' → step2 s s'.
+intros. induction H0; try constructor. assert (Φ ++ l ↦ cl (close (lam b) e) e'
+:: Υ = replace beq_nat l (cl (close (lam b) e) e') (Φ ++ l↦(cl c e') :: Υ)).
+rename c into C. rewrite replace_inf with (c:=(cl C e')).  reflexivity.
+assumption.  rewrite H0. apply Upd2 with (c':=c). apply unique_domain_lookup.
+assumption. exists Φ, Υ. reflexivity. assumption. apply Abs2 with (p:=p).
+assumption. Qed. 
+
+(*
+Lemma lookup_unique_domain {b} : ∀ xs ys, unique (domauin
+  unique (domain (Φ ++ l ↦ c :: Ψ)) →
+  Φ ++ l ↦ c :: Ψ = Φ' ++ l ↦ c' :: Ψ' → Φ = Φ' ∧ Ψ = Ψ' ∧ c = c'.
+intros. remember (domain (Φ ++ l↦c :: Ψ)). generalize dependent Φ. generalize
+dependent c'. generalize dependent Ψ. induction H; intros; subst. unfold domain
+in Heql0. rewrite map_app in Heql0. simpl in Heql0. apply app_cons_not_nil in
+Heql0. inversion Heql0. unfold domain in H. rewrite map_app in H. induction Φ.
+simpl in H0. induction Φ'. inversion H0. subst. auto.  inversion H0. subst.
+simpl in H. inversion H; subst. unfold domain in H2. rewrite map_app in H2.
+rewrite in_app_iff in H2. apply or_imp in H2. destruct H2.  simpl in H2. apply
+or_imp in H2. destruct H2. specialize (H2 eq_refl). inversion H2. inversion H0.
+induction Φ'. inversion H0. subst. destruct H. inversion H0.  inversion H0.
+subst. remember (Φ ++ l↦c :: Ψ). apply eq_inf_indomain in Heql0.  apply H in
+Heql0. inversion Heql0. inversion H0. subst. split. apply f_equal.  symmetry in
+H0. apply app_eq_unit in H0. destruct H0. destruct H0. subst. inversion H1.
+subst. auto. inversion H0.  subst. inversion H2. inversion H0. inversion_clear
+H; subst. simpl in H1. apply or_imp in H1. destruct H1. apply ucons with (v:=c)
+in H1. simpl in IHΨ.  specialize (IHΨ H1). induction Φ'. inversion H0. subst.
+auto. simpl in H0.  inversion H0. subst. apply eq_inf_indomain in H5.  simpl in
+IHΦ'. destruct H5.  crush. inversion H1. crush. inversion H0. apply
+eq_inf_indomain in H5. apply IHΦ'.  simpl in H0. 
+
+unfold not in H1.
+simpl in H1. destruct incrush. apply app_eq_unit in H0.  
+  
+Lemma step_determ : deterministic (λ c c', unique_domain (st_heap c) ∧ step' c c').  
+unfold deterministic. intros. crush. inversion H2; inversion H3; subst; crush;
+auto. inversion H5; subst. 
+
+Lemma normalize2_determ : deterministic normalize2.  
 
 
-(* Step as a function *
+ Step as a function *
+Lemma well_formed_step : ∀ s s', well_formed s → s →s s' → well_formed s'. 
+intros.  induction H0. apply well_formed_inf. 
 
 Lemma well_formed_lookup : ∀ l h c e, well_formed_heap h → lookup eq_nat_dec l h = Some (cl c e) →
   closed_under c h.
